WIP

src/Bedrock/Field/Translation/Proofs/ValidComputable/Expr.v
@@ -1,3 +1,4 @@
+Require Import Coq.derive.Derive.
 Require Import Coq.ZArith.ZArith.
 Require Import Coq.Bool.Bool.
 Require Import Coq.Lists.List.
@@ -12,14 +13,20 @@ Require Import Crypto.Language.API.
 Require Import Crypto.Util.Decidable.
 Require Import Crypto.Util.ZRange.
 Require Import Crypto.Util.Tactics.BreakMatch.
+Require Import Crypto.Util.Tactics.Head.
 Require Import Crypto.Util.ZUtil.Tactics.LtbToLt.
 Require Import Crypto.Util.Bool.Reflect.
+Require Import Crypto.Util.ListUtil.FoldBool.
+Require Import Crypto.Util.Tactics.DestructHead.
+Require Import Crypto.Util.HProp.
+Require Import Crypto.Util.Tactics.UniquePose.
 Local Open Scope Z_scope.
 Local Open Scope bool_scope.
 
 Import API.Compilers.
 Import Wf.Compilers.expr.
 Import Types.Notations.
+Import Inversion.Compilers.
 
 Section Expr.
   Context {p : Types.parameters} {p_ok : @ok p}.
@@ -28,6 +35,425 @@ Section Expr.
   Local Existing Instance Types.rep.listZ_local.
   Local Instance sem_ok : Semantics.parameters_ok semantics
     := semantics_ok.
+
+  Ltac intros_do_revert tac :=
+    lazymatch goal with
+    | [ |- forall x : _, _ ] => let x' := fresh in intro x'; intros_do_revert tac; revert x'
+    | _ => tac ()
+    end.
+
+  Ltac split_lists :=
+    refine (@nth_error_true_fold_left_orb_true _ _ _ _);
+    [ > cbn [nth_error];
+      repeat lazymatch goal with
+             | [ |- nth_error (_ :: _) ?n = Some true ]
+               => is_evar n;
+                  let n' := open_constr:(S _) in
+                  unify n n';
+                  cbn [nth_error]
+             | [ |- nth_error ?ev ?n = Some true ]
+               => let ev := head ev in
+                  is_evar ev; is_evar n;
+                  let EV := fresh in
+                  pose ev as EV;
+                  instantiate (1:=ltac:(intros_do_revert ltac:(fun _ => refine (cons _ _)))) in (value of EV); clear EV; cbv beta;
+                  unify n O;
+                  cbn [nth_error]; apply f_equal
+             end .. ].
+
+  Ltac get_last ls :=
+    lazymatch ls with
+    | cons _ ?ls => get_last ls
+    | _ => ls
+    end.
+  Ltac handle_first_var lhs :=
+    lazymatch lhs with
+    | ?ev ?x ?y => handle_first_var (ev x)
+    | ?ev ?e
+      => is_evar ev;
+         (tryif is_var e
+           then instantiate (1:=ltac:(intro)); cbv beta
+           else instantiate (1:=ltac:(let e := fresh "e" in intro e; case e; clear e)); cbv beta iota in * )
+    end.
+  Ltac split_recr valid_expr_bool :=
+    lazymatch goal with
+    | [ H : valid_expr_bool _ _ _ = true |- _ ]
+      => instantiate (1:=ltac:(let e := fresh "e" in intro e; refine (andb _ _); revert e));
+         cbv beta; refine (andb_true_intro _); split;
+         [ clear H; split_recr valid_expr_bool | clear -H ]
+    | _ => instantiate (1:=fun _ => true); reflexivity
+    end.
+  Ltac get_first_arg f :=
+    lazymatch f with
+    | ?f ?x
+      => lazymatch f with
+         | ?f' _ => get_first_arg f
+         | _ => x
+         end
+    end.
+  Ltac terms_intersect x y :=
+    match x with
+    | context[?x'] => match y with
+                      | context[x'] => constr:(true)
+                      end
+    | _ => constr:(false)
+    end.
+  Ltac destruct_to_instantiate_with valid_expr_bool H x :=
+    repeat lazymatch goal with
+           | [ |- ?lhs = true ]
+             => let x' := get_first_arg lhs in
+                let inter := terms_intersect x x' in
+                lazymatch inter with
+                | false => instantiate (1:=ltac:(intro)); cbv beta
+                | true => handle_first_var lhs
+                end
+           end;
+    (instantiate (1:=ltac:(refine (valid_expr_bool _ _ _); clear valid_expr_bool)));
+    refine H.
+  Ltac instantiate_non_recr valid_expr_bool :=
+    clear dependent valid_expr_bool;
+    repeat match goal with
+             [ H : valid_expr _ _ |- _ ] => clear H
+           end;
+    repeat lazymatch goal with
+           | [ |- ?lhs = true ]
+             => handle_first_var lhs
+           end;
+    repeat lazymatch goal with
+           | [ H : _ |- _ ]
+             => lazymatch type of H with
+                | _ = true
+                  => refine (andb_true_intro _); split;
+                     [ clear H
+                     | refine H ]
+                | ?T
+                  => lazymatch type of T with
+                     | Prop
+                       => refine (andb_true_intro _); split;
+                          [ clear H
+                          | solve [ refine (unreflect_bool H) ]
+                            || (idtac "could not reflect:" T; fail) ]
+                     | _ => clear H
+                     end
+                end
+           | _ => instantiate (1:=true); reflexivity
+           end.
+  Ltac unfold_valid_expr_bool valid_expr_bool :=
+    cbv [valid_expr_bool]; fold valid_expr_bool; clearbody valid_expr_bool.
+  Ltac finish_non_recr_instantiation valid_expr_bool :=
+    instantiate (1:=ltac:(let e := fresh "e" in
+                          intro e;
+                          refine (andb _ _);
+                          [ clear valid_expr_bool
+                          | ];
+                          revert e));
+    cbv beta;
+    (refine (andb_true_intro _); split;
+     [ instantiate_non_recr valid_expr_bool; shelve
+     | split_recr valid_expr_bool ]).
+  Ltac finish_recr_instantiation valid_expr_bool :=
+    lazymatch goal with
+    | [ H : valid_expr_bool _ _ ?x = true |- _ ]
+      => destruct_to_instantiate_with valid_expr_bool H x
+    end.
+  Ltac get_valid_expr_bool :=
+    lazymatch reverse goal with
+    | [ valid_expr_bool : forall t, bool -> API.expr t -> bool |- _ ]
+      => valid_expr_bool
+    end.
+  Ltac get_valid_expr_bool_correct valid_expr_bool :=
+    lazymatch goal with
+    | [ valid_expr_bool_correct : forall t rc e, valid_expr_bool t rc e = true -> valid_expr rc e |- _ ] => valid_expr_bool_correct
+    end.
+  Ltac fill_valid_expr_bool_after_split_lists :=
+    unshelve (
+        let valid_expr_bool := get_valid_expr_bool in
+        finish_non_recr_instantiation valid_expr_bool;
+        finish_recr_instantiation valid_expr_bool
+      );
+    try (intros; exact false).
+  Ltac fill_valid_expr_bool :=
+    (let valid_expr_bool := get_valid_expr_bool in
+     unfold_valid_expr_bool valid_expr_bool);
+    split_lists;
+    fill_valid_expr_bool_after_split_lists.
+
+  Ltac early_safe_step1 :=
+    first [ progress cbn [andb] in *
+          | match goal with
+            | [ |- false = true -> _ ] => intro
+            | [ |- true = false -> _ ] => intro
+            | [ H : true = false |- _ ] => exfalso; clear -H; discriminate
+            | [ H : false = true |- _ ] => exfalso; clear -H; discriminate
+            end ].
+  Ltac early_safe_step2 :=
+    first [ match goal with
+            | [ |- context[match ?e with _ => _ end] ] => is_var e; destruct e
+            | [ H : context[match ?e with _ => _ end] |- _ ] => is_var e; destruct e
+            | [ veb := _ : bool |- _ ] => clearbody veb
+            end ].
+  Ltac early_safe_step := first [ early_safe_step1 | early_safe_step2 ].
+  Ltac early_step valid_expr_bool valid_expr_bool_correct :=
+    first [ early_safe_step1
+          | match goal with
+            | [ |- context[valid_expr_bool ?t ?rc ?e] ]
+              => unique pose proof (valid_expr_bool_correct t rc e);
+                 let veb := fresh "veb" in
+                 set (veb := valid_expr_bool t rc e) in *
+            | [ |- context[?e] ]
+              => lazymatch e with
+                 | context[valid_expr_bool]
+                   => match e with
+                      | context[match ?e with _ => _ end] => is_var e; destruct e
+                      end
+                 end
+            end
+          | early_safe_step2 ].
+
+  Definition valid_expr_bool_package
+    : { valid_expr_bool_step
+        : ((forall {t} (rc : bool) (e : API.expr t), bool)
+           -> (forall {t} (rc : bool) (e : API.expr t), bool))
+          & { valid_expr_bool
+              : (forall {t} (rc : bool) (e : API.expr t), bool)
+                & (forall {t} (rc : bool) (e : API.expr t),
+                  (*reflect (valid_expr rc e) (valid_expr_bool t rc e)*)
+                  valid_expr rc e -> valid_expr_bool t rc e = true)
+                  * (forall {t} (rc : bool) (e : API.expr t),
+                        @valid_expr_bool t rc e = @valid_expr_bool_step (@valid_expr_bool) t rc e) }%type }.
+  Proof using Type.
+    clear p_ok.
+    unshelve
+      (simple refine (let valid_expr_bool_step
+                          : (forall {t} (rc : bool) (e : API.expr t), bool)
+                            -> (forall {t} (rc : bool) (e : API.expr t), bool)
+                          := fun valid_expr_bool t rc e
+                             => fold_left orb _ false in
+                      let valid_expr_bool := (fix valid_expr_bool {t} (rc : bool) (e : API.expr t) {struct e} : bool := valid_expr_bool_step (@valid_expr_bool) t rc e) in
+                      let valid_expr_bool_eta : forall t rc e, @valid_expr_bool t rc e = valid_expr_bool_step (@valid_expr_bool) t rc e
+                          := _ in
+                      (*let valid_expr_bool_step_correct'
+                          : (forall (t : API.type) (rc : bool) (e : API.expr t),
+                                @valid_expr_bool t rc e = true -> valid_expr rc e)
+                            -> forall (t : API.type) (rc : bool) (e : API.expr t),
+                              valid_expr_bool_step (@valid_expr_bool) t rc e = true -> valid_expr rc e
+                          := _ in
+                      let valid_expr_bool_step_correct := _ in*)
+                      let valid_expr_bool_correct := _ in
+                      existT
+                        _ (@valid_expr_bool_step)
+                        (existT
+                           _ (@valid_expr_bool)
+                           ((fun t rc e
+                             => (*iff_reflect
+                                  _ _
+                                  (conj*) (valid_expr_bool_correct t rc e)
+                                        (*((fix valid_expr_bool_correct' {t} (rc : bool) (e : API.expr t) {struct e} := valid_expr_bool_step_correct (@valid_expr_bool_correct') t rc e) t rc e))*)),
+                            valid_expr_bool_eta)));
+       [ revert valid_expr_bool t rc e
+       | clear -p; intros ? ? e; destruct e; cbn [valid_expr_bool]; reflexivity
+       (*| clearbody valid_expr_bool_eta
+       | clearbody valid_expr_bool_eta valid_expr_bool_step_correct';
+         let H := fresh in
+         intro H; specialize (valid_expr_bool_step_correct' H);
+         intros t rc e;
+         pose e as e';
+         destruct e;
+         let e' := (eval cbv delta [e'] in e') in
+         refine (valid_expr_bool_step_correct' _ rc e')*)
+       | (*clear valid_expr_bool_step_correct' valid_expr_bool_step_correct;*)
+         clearbody valid_expr_bool_eta;
+         intros t rc e H;
+         induction H;
+         rewrite valid_expr_bool_eta; clear valid_expr_bool_eta;
+         clearbody valid_expr_bool;
+         cbv [valid_expr_bool_step];
+         clear valid_expr_bool_step;
+         split_lists;
+         lazymatch goal with
+         | [ |- ?ev ?veb ?t ?rc ?e = true ]
+           => let subcall := fresh "subcall" in
+              let ty := type of ev in
+              let H := fresh in
+              let rcv := lazymatch rc with
+                         | true => constr:(Some true)
+                         | false => constr:(Some false)
+                         | _ => constr:(@None bool)
+                         end in
+              simple refine (let subcall : ty := _ in
+                             let H : subcall veb t rc e = true := _ in
+                             _);
+              [ clear -p;
+                let t := fresh "t" in
+                let rc := fresh "rc" in
+                let e := fresh "e" in
+                intros valid_expr_bool t rc e;
+                lazymatch rcv with
+                | Some true => refine (andb rc _)
+                | Some false => refine (andb (negb rc) _)
+                | None => idtac
+                end;
+                revert e; shelve
+              | subst subcall; cbv beta;
+                lazymatch goal with
+                | [ |- andb _ _ = true ] => apply andb_true_intro; split; [ reflexivity | ]
+                | [ |- _ = true ] => idtac
+                end;
+                fill_valid_expr_bool_after_split_lists
+              | let T := type of subcall in
+                let subcall' := fresh "subcall'" in
+                simple refine (let subcall' : T := _ in
+                               _);
+                [ clear -subcall;
+                  let subcall_body := (eval cbv beta iota delta [subcall] in subcall) in
+                  clear subcall;
+                  transparent_abstract (exact subcall_body)
+                | let subcallv := (eval cbv delta [subcall'] in subcall') in
+                  instantiate (1:=subcallv);
+                  replace subcallv with subcall by reflexivity;
+                  refine H ] ]
+         end ]).
+    intros; exact nil.
+  Defined.
+
+  Definition valid_expr_bool_step
+    : forall (valid_expr_bool : forall {t} (rc : bool) (e : API.expr t), bool)
+             {t} (rc : bool) (e : API.expr t), bool
+    := Eval cbv [projT1 valid_expr_bool_package] in projT1 valid_expr_bool_package.
+
+  Fixpoint valid_expr_bool {t} (rc : bool) (e : API.expr t) {struct e} : bool
+    := @valid_expr_bool_step (@valid_expr_bool) t rc e.
+
+  Lemma valid_expr_bool_eta {t} (rc : bool) (e : API.expr t)
+    : valid_expr_bool rc e = @valid_expr_bool_step (@valid_expr_bool) t rc e.
+  Proof using Type. now destruct e. Qed.
+
+  Lemma valid_expr_bool_impl2
+    : forall {t} (rc : bool) (e : API.expr t),
+      valid_expr rc e -> valid_expr_bool rc e = true.
+  Proof using Type. exact (fst (projT2 (projT2 valid_expr_bool_package))). Qed.
+
+  Definition valid_expr_bool_impl1_step
+             (valid_expr_bool_correct
+              : forall {t} (rc : bool) (e : API.expr t),
+                 valid_expr_bool rc e = true -> valid_expr rc e)
+             {t} (rc : bool) (e : API.expr t)
+    : valid_expr_bool rc e = true -> valid_expr rc e.
+  Proof using Type.
+    clear p_ok.
+    rewrite valid_expr_bool_eta.
+    cbv [valid_expr_bool_step].
+    lazymatch goal with
+    | [ |- fold_left orb ?ls ?b = true -> _ ]
+      => induction_fold_left_orb_true ls b
+    end.
+    all: lazymatch goal with
+         | [ |- false = true -> _ ]
+           => let H := fresh in
+              intro H; exfalso; clear -H; discriminate
+         | [ |- ?lhs = true -> valid_expr _ _ ]
+           => let h := head lhs in
+              cbv [h]
+         end.
+    Time
+      all: intro;
+  repeat match goal with
+         | [ H : andb _ _ = true |- _ ] => apply andb_prop in H; destruct H
+    end.
+    Time all: let valid_expr_bool_correct := get_valid_expr_bool_correct (@valid_expr_bool) in
+              repeat (let H := match goal with
+                               | [ H : ?lhs = true |- _ ]
+                                 => let __ := match lhs with context[valid_expr_bool] => idtac end in
+                                    H
+                               end in
+                      let H' := fresh in
+                      eassert (H' : _);
+                     [ instantiate (1:=ltac:(clear H));
+                     repeat match goal with
+                            | [ H' : _ |- _ ] => tryif first [ constr_eq H H' | constr_eq H' valid_expr_bool_correct ] then fail else clear H'
+                            end;
+                     repeat match type of H with
+                            | context[match ?e with _ => _ end]
+                              => is_var e;
+                     instantiate (1:=ltac:(destruct e)); destruct e
+                     | false = true => refine (_ : False); clear -H; discriminate
+                       end;
+                     lazymatch type of H with
+                     | @valid_expr_bool _ _ _ = true
+                       => refine (valid_expr_bool_correct _ _ _ H)
+                     | ?T => fail 1 "Leftover:" T
+                     end
+                     | clear H ]).
+    all: clear valid_expr_bool_correct.
+    Time all:
+      time
+        abstract (
+          time repeat early_safe_step;
+        time repeat first [ early_safe_step
+                          | progress subst
+                          | match goal with
+                            | [ H : negb ?x = ?y |- _ ]
+                              => let H' := fresh in
+                                 assert (H' : x = negb y) by (clear -H; now destruct x, y);
+                          cbn [negb] in H'; clear H
+                            end
+                          | expr.invert_match_step
+                          | match goal with
+                            | [ H : context[match ?x with _ => _ end ] |- _ ]
+                              => is_var x;
+                          lazymatch type of x with
+                          | ?F ?t
+                            => lazymatch type of t with
+                               | API.type
+                                 => type.invert_one x; subst; inversion_type
+                            end
+                            end
+                            end
+                          | match goal with
+                            | [ H : ?x = ?x |- _ ] => clear H
+                            | [ H : ?x = ?v |- _ ]
+                              => let b := lazymatch v with true => x | false => constr:(negb x) end in
+                                 lazymatch constr:(@id (reflect _ b) _) with
+                                 | @id (reflect (?x = ?x) _) _
+                                   => clear H
+                                 | @id (reflect ?P _) ?lem
+                                   => unique assert P;
+                          [ let H' := fresh in
+                            pose proof lem as H'; rewrite H in H'; cbn [negb] in H';
+                          inversion H'; assumption
+                          | ]
+                            end
+                            end ];
+    (* Tactic call ran for 2.641 secs (2.628u,0.011s) (success)
+Tactic call ran for 23.769 secs (23.632u,0.135s) (success)
+Tactic call ran for 1.041 secs (1.029u,0.012s) (success)
+Tactic call ran for 1.06 secs (1.048u,0.011s) (success)
+Tactic call ran for 1.602 secs (1.598u,0.003s) (success)
+Tactic call ran for 0.002 secs (0.002u,0.s) (success)
+Tactic call ran for 0. secs (0.u,0.s) (success)
+Tactic call ran for 0. secs (0.u,0.s) (success)
+Tactic call ran for 8.624 secs (8.58u,0.043s) (success)
+Tactic call ran for 5.875 secs (5.843u,0.031s) (success)
+Tactic call ran for 5.916 secs (5.916u,0.s) (success)
+Tactic call ran for 18.244 secs (18.244u,0.s) (success)
+Tactic call ran for 17.057 secs (17.057u,0.s) (success)
+Tactic call ran for 6.049 secs (6.049u,0.s) (success)
+Tactic call ran for 12.284 secs (12.284u,0.s) (success)
+Tactic call ran for 0.887 secs (0.887u,0.s) (success)
+Tactic call ran for 0.649 secs (0.649u,0.s) (success)
+
+Finished transaction in 105.706 secs (105.453u,0.252s) (successful)
+     *)
+        constructor; solve [ eauto ]
+        ).
+    (* Tactic call ran for 282.124 secs (281.901u,0.224s) (success) *)
+    Time Defined.
+  (*Finished transaction in 76.9 secs (76.9u,0.s) (successful)*)
+
+  Time Fixpoint valid_expr_bool_impl1 {t} (rc : bool) (e : API.expr t) {struct e}
+    : valid_expr_bool rc e = true -> valid_expr rc e
+    := @valid_expr_bool_impl1_step (@valid_expr_bool_impl1) t rc e.
+  (* Finished transaction in 0.387 secs (0.387u,0.s) (successful) *)
 
   Definition is_fst_snd_ident {t} (i : ident.ident t) : bool :=
     match i with
@@ -114,6 +540,31 @@ Section Expr.
     match e with
     | expr.Ident _ (ident.Literal base.type.Z n) =>
       is_bounded_by_bool n width_range
+    | _ => false
+    end.
+
+  Definition is_lnot_modulo_ident {t} (i : ident.ident t) :=
+    match i with
+    | ident.Z_lnot_modulo => true
+    | _ => false
+    end.
+  Definition is_lnot_modulo_ident_expr
+             {t} (e : @API.expr (fun _ => unit) t) :=
+    match e with
+    | expr.Ident
+        (type.arrow type_Z (type.arrow type_Z type_Z))
+        i => is_lnot_modulo_ident i
+    | _ => false
+    end.
+  Definition valid_expr_lnot_modulo_bool {t} (require_casts : bool)
+           (e : @API.expr (fun _ => unit) t) : bool :=
+    match e with
+    | expr.App
+        type_Z (type.arrow type_Z (type.arrow type_Z type_Z))
+        f (expr.Ident _ (ident.Literal base.type.Z m)) =>
+      (is_lnot_modulo_ident_expr f)
+        && (negb require_casts)
+        && Z.eqb (2^Z.log2 m) m
     | _ => false
     end.
 
@@ -1151,6 +1602,8 @@ Section Expr.
         destruct (translate_binop i)
       end; cbn [andb]; congruence. }
   Qed.
+
+
 
   Lemma valid_expr_bool_iff {t} (e : API.expr (type.base t)) :
     forall rc,
